Verified Paxos protocol lemmas, except for this key lemma:
Given a set of natural numbers W s.t. all s ∈ W have s < n,
then size W < n.
I.e. there are only n distinct natural numbers that are less than n.

Had to do some interesting proof to update several pieces of a big_sepS
all at once.

src/program_proof/mpaxos/ghost_proof.v
@@ -71,9 +71,12 @@ Definition own_commit γ σ : iProp Σ :=
 Definition is_ghost_lb γ σ : iProp Σ :=
   own γ.(mp_state_gn) (◯ML (σ : list (leibnizO (EntryType)))).
 
-(* FIXME: this definition needs to only require a quorum *)
+(* This definition needs to only require a quorum *)
 Definition committed_by epoch σ : iProp Σ :=
-  ∀ γsrv, ⌜γsrv ∈ config⌝ → is_accepted_lb γsrv epoch σ.
+  ∃ (W:gset nat),
+  ⌜(∀ s, s ∈ W → s < length config)⌝ ∗
+  ⌜2 * (size W) > length config⌝ ∗
+  ([∗ list] s0↦γsrv' ∈ config, ⌜s0 ∈ W⌝ → is_accepted_lb γsrv' epoch σ).
 
 Definition old_proposal_max γsys epoch σ : iProp Σ := (* persistent *)
   □(∀ epoch_old σ_old,
@@ -106,11 +109,6 @@ Definition is_proposal_facts γ epoch σ: iProp Σ :=
   old_proposal_max γ epoch σ ∗
   is_proposal_valid γ σ.
 
-(* FIXME: these definitions need to change *)
-Definition own_escrow_toks γsrv epoch : iProp Σ :=
-  [∗ set] epoch' ∈ (fin_to_set u64), ⌜int.nat epoch' ≤ int.nat epoch⌝ ∨ own_vote_tok γsrv epoch'
-.
-
 Record MPaxosState :=
   mkMPaxosState
     {
@@ -119,11 +117,39 @@ Record MPaxosState :=
       mp_log:list EntryType ;
     }.
 
-Definition own_replica_ghost γsys γsrv (st:MPaxosState) : iProp Σ.
-Admitted.
+Definition is_accepted_upper_bound γsrv log (acceptedEpoch newEpoch:u64) : iProp Σ :=
+  ∃ logPrefix,
+  ⌜logPrefix ⪯ log⌝ ∗
+  is_accepted_ro γsrv acceptedEpoch logPrefix ∗
+  □ (∀ epoch', ⌜int.nat acceptedEpoch < int.nat epoch'⌝ -∗
+            ⌜int.nat epoch' < int.nat newEpoch⌝ -∗
+            is_accepted_ro γsrv epoch' [])
+.
 
-Definition own_leader_ghost γsys (st:MPaxosState): iProp Σ.
-Admitted.
+
+Definition own_replica_ghost γsys γsrv (st:MPaxosState) : iProp Σ :=
+  "#Hprop_lb" ∷ is_proposal_lb γsys st.(mp_acceptedEpoch) st.(mp_log) ∗
+  "#Hprop_facts" ∷ is_proposal_facts γsys st.(mp_acceptedEpoch) st.(mp_log) ∗
+  "#Hacc_lb" ∷ is_accepted_lb γsrv st.(mp_acceptedEpoch) st.(mp_log) ∗
+  "%HepochIneq" ∷ ⌜int.nat st.(mp_acceptedEpoch) ≤ int.nat st.(mp_epoch)⌝ ∗
+
+  "Hacc" ∷ (if (decide (int.nat st.(mp_acceptedEpoch) = int.nat st.(mp_epoch))) then
+                  own_accepted γsrv st.(mp_epoch) st.(mp_log)
+                else
+                 own_accepted γsrv st.(mp_epoch) []) ∗
+   (* XXX: could combine this with the previous proposition *)
+  "#Hacc_ub" ∷ (⌜int.nat st.(mp_acceptedEpoch) < int.nat st.(mp_epoch)⌝ →
+                 is_accepted_upper_bound γsrv st.(mp_log) st.(mp_acceptedEpoch) st.(mp_epoch)) ∗
+
+
+  "Hunused" ∷ ([∗ set] e ∈ (fin_to_set u64), (⌜int.nat e > int.nat st.(mp_epoch)⌝ → own_accepted γsrv e [])) ∗
+  "Hvotes" ∷ ([∗ set] epoch' ∈ (fin_to_set u64), ⌜int.nat epoch' ≤ int.nat st.(mp_epoch)⌝ ∨ own_vote_tok γsrv epoch')
+.
+
+Definition own_leader_ghost γsys (st:MPaxosState): iProp Σ :=
+  "Hprop" ∷ own_proposal γsys st.(mp_epoch) st.(mp_log) ∗
+  "#Hprop_facts" ∷ is_proposal_facts γsys st.(mp_epoch) st.(mp_log)
+.
 
 Lemma ghost_leader_propose γsys st entry :
   own_leader_ghost γsys st -∗
@@ -136,14 +162,168 @@ Lemma ghost_leader_propose γsys st entry :
   is_proposal_facts γsys st.(mp_epoch) (st.(mp_log) ++ [entry])
 .
 Proof.
-Admitted.
+  iNamed 1.
+  iIntros "Hlc Hupd".
+
+  iMod (own_update with "Hprop") as "Hprop".
+  {
+    apply singleton_update.
+    apply csum_update_r.
+    apply mono_list_update.
+    instantiate (1:=(st.(mp_log) ++ [entry])).
+    apply prefix_app_r.
+    done.
+  }
+
+  iDestruct (own_mono _ _
+               {[ st.(mp_epoch) := Cinr (◯ML _) ]}
+              with "Hprop") as "#Hprop_lb".
+  {
+    apply singleton_mono.
+    apply Cinr_included.
+    apply mono_list_included.
+  }
+
+  iFrame "∗#".
+
+  iAssert (|={⊤}=> is_proposal_facts γsys st.(mp_epoch) (st.(mp_log) ++ [entry]))%I with "[Hupd Hlc]" as ">#Hvalid2".
+  {
+    iDestruct "Hprop_facts" as "(Hmax & Hvalid)".
+    iSplitL "".
+    { (* old proposal max *)
+      iModIntro.
+      unfold old_proposal_max.
+      iModIntro.
+      iIntros.
+      iAssert (⌜σ_old ⪯ st.(mp_log)⌝)%I as "%Hprefix".
+      {
+        iApply "Hmax".
+        {
+          done.
+        }
+        { iFrame "#". }
+      }
+      iPureIntro.
+      apply prefix_app_r.
+      done.
+    }
+
+    iAssert (|={⊤}=> is_valid_inv γsys st.(mp_log) entry)%I with "[Hupd Hlc]" as ">#Hinv".
+    {
+      iMod (inv_alloc with "[Hupd Hlc]") as "$".
+      {
+        iNext.
+        iLeft.
+        iFrame.
+      }
+      done.
+    }
+    (* prove is_proposal_valid γ (σ ++ [op]) *)
+    iModIntro.
+    iModIntro.
+    iIntros (σ') "%Hσ' Hσ'".
+    assert (σ' ⪯ st.(mp_log) ∨ σ' = (st.(mp_log) ++ [entry])) as [Hprefix_old|Hlatest].
+    { (* TODO: list_solver. *)
+      (* TODO: copy/paste from pb_ghost *)
+      assert (Hlen := Hσ').
+      apply prefix_length in Hlen.
+      assert (length σ' = length (st.(mp_log) ++ [entry]) ∨ length σ' < length (st.(mp_log) ++ [entry])) as [|] by word.
+      {
+        right.
+        apply list_prefix_eq; eauto.
+        lia.
+      }
+      {
+        left.
+        rewrite app_length in H.
+        simpl in H.
+        apply list_prefix_bounded.
+        { word. }
+        intros.
+        assert (st.(mp_log) !! i = (st.(mp_log) ++ [entry]) !! i).
+        {
+          rewrite lookup_app_l.
+          { done. }
+          { word. }
+        }
+        rewrite H1.
+        apply list_prefix_forall.
+        { done. }
+        { done. }
+      }
+    }
+    {
+      iMod ("Hvalid" $! σ' Hprefix_old with "Hσ'") as "Hσ".
+      iInv "Hinv" as "Hi" "Hclose".
+      iDestruct "Hi" as "[Hupd|#>Hlb]"; last first.
+      {
+        iDestruct (own_valid_2 with "Hσ Hlb") as "%Hvalid".
+        exfalso.
+        rewrite mono_list_both_dfrac_valid_L in Hvalid.
+        destruct Hvalid as [_ Hvalid].
+        apply prefix_length in Hvalid.
+        rewrite app_length in Hvalid.
+        simpl in Hvalid.
+        word.
+      }
+      iDestruct "Hupd" as "[>Hlc Hupd]".
+      iMod (lc_fupd_elim_later with "Hlc Hupd" ) as "Hupd".
+      iMod (fupd_mask_subseteq (⊤∖↑ghostN)) as "Hmask".
+      {
+        assert ((↑sysN:coPset) ⊆ (↑ghostN:coPset)).
+        { apply nclose_subseteq. }
+        assert ((↑opN:coPset) ⊆ (↑ghostN:coPset)).
+        { apply nclose_subseteq. }
+        set_solver.
+      }
+      iMod "Hupd".
+      iDestruct "Hupd" as (?) "[Hghost Hupd]".
+      iDestruct (own_valid_2 with "Hghost Hσ") as %Hvalid.
+      rewrite mono_list_auth_dfrac_op_valid_L in Hvalid.
+      destruct Hvalid as [_ ->].
+      iCombine "Hghost Hσ" as "Hσ".
+      iMod (own_update with "Hσ") as "Hσ".
+      {
+        apply (mono_list_update (st.(mp_log) ++ [entry] : list (leibnizO EntryType))).
+        by apply prefix_app_r.
+      }
+      iEval (rewrite -Qp.half_half) in "Hσ".
+      rewrite -dfrac_op_own.
+      rewrite mono_list_auth_dfrac_op.
+      iDestruct "Hσ" as "[Hσ Hcommit]".
+      iSpecialize ("Hupd" with "[] Hσ").
+      { done. }
+      iMod "Hupd".
+
+      rewrite mono_list_auth_lb_op.
+      iDestruct "Hcommit" as "[Hcommit #Hlb]".
+      iMod "Hmask".
+      iMod ("Hclose" with "[]").
+      {
+        iNext.
+        iRight.
+        iFrame "Hlb".
+      }
+      iModIntro.
+      iFrame.
+    }
+    {
+      rewrite Hlatest.
+      by iFrame.
+    }
+  }
+  iModIntro.
+  iFrame "#".
+Qed.
 
 Lemma ghost_replica_get_lb γsys γsrv st :
   own_replica_ghost γsys γsrv st -∗
   is_accepted_lb γsrv st.(mp_acceptedEpoch) st.(mp_log).
 Proof.
-Admitted.
+  by iNamed 1.
+Qed.
 
+(* Similar to ghost_accept in pb_ghost.v *)
 Lemma ghost_replica_accept_same_epoch γsys γsrv st epoch' log' :
   int.nat st.(mp_epoch) ≤ int.nat epoch' →
   int.nat st.(mp_acceptedEpoch) = int.nat epoch' →
@@ -155,7 +335,61 @@ Lemma ghost_replica_accept_same_epoch γsys γsrv st epoch' log' :
   ⌜st.(mp_epoch) = epoch'⌝ ∗
   own_replica_ghost γsys γsrv (mkMPaxosState epoch' epoch' log').
 Proof.
-Admitted.
+  intros Hineq1 Hineq2 Hlen.
+  iNamed 1.
+  iIntros "#Hprop_lb2 #Hprop_facts2".
+  iAssert (⌜st.(mp_epoch) = epoch'⌝)%I as "%HepochEq".
+  { iPureIntro. word. }
+  iFrame "%".
+  destruct (decide _); last first.
+  {
+    exfalso. naive_solver.
+  }
+
+  iDestruct (own_valid_2 with "Hprop_lb Hprop_lb2") as %Hcomp.
+  rewrite -HepochEq in Hcomp.
+  replace (st.(mp_acceptedEpoch)) with (st.(mp_epoch)) in Hcomp by word.
+
+  rewrite singleton_op singleton_valid in Hcomp.
+  rewrite -Cinr_op Cinr_valid in Hcomp.
+  rewrite mono_list_lb_op_valid_L in Hcomp.
+
+  assert (st.(mp_log)⪯log').
+  {
+    destruct Hcomp as [Hbad|Hcomp]; first done.
+    enough (log'=st.(mp_log)) by naive_solver.
+    by apply list_prefix_eq.
+  }
+  rewrite -e.
+
+  iMod (own_update with "Hacc") as "Hacc".
+  {
+    apply singleton_update.
+    apply mono_list_update.
+    instantiate (1:=log').
+    done.
+  }
+  iClear "Hacc_lb".
+  iDestruct (own_mono _ _
+               {[ st.(mp_epoch) := (◯ML _) ]}
+              with "Hacc") as "#Hacc_lb".
+  {
+    apply singleton_mono.
+    apply mono_list_included.
+  }
+
+  iModIntro.
+  replace st.(mp_epoch) with epoch' by word.
+  replace st.(mp_acceptedEpoch) with epoch' by word.
+  unfold own_replica_ghost.
+  simpl.
+  rewrite decide_True; last done.
+  iFrame "∗#".
+  iSplitL; first done.
+  iIntros (?).
+  exfalso.
+  lia.
+Qed.
 
 Lemma ghost_replica_accept_same_epoch_old γsys γsrv st epoch' log' :
   int.nat st.(mp_epoch) ≤ int.nat epoch' →
@@ -165,7 +399,43 @@ Lemma ghost_replica_accept_same_epoch_old γsys γsrv st epoch' log' :
   is_proposal_lb γsys epoch' log' -∗
   is_accepted_lb γsrv epoch' log'.
 Proof.
-Admitted.
+  intros Hineq1 Heq2 Hlen.
+  iNamed 1.
+  iIntros "#Hprop_lb2".
+  iAssert (⌜st.(mp_epoch) = epoch'⌝)%I as "%HepochEq".
+  { iPureIntro. word. }
+  iFrame "%".
+  destruct (decide _); last first.
+  {
+    exfalso. naive_solver.
+  }
+
+  iDestruct (own_valid_2 with "Hprop_lb Hprop_lb2") as %Hcomp.
+  rewrite -HepochEq in Hcomp.
+  replace (st.(mp_acceptedEpoch)) with (st.(mp_epoch)) in Hcomp by word.
+
+  rewrite singleton_op singleton_valid in Hcomp.
+  rewrite -Cinr_op Cinr_valid in Hcomp.
+  rewrite mono_list_lb_op_valid_L in Hcomp.
+
+  assert (log'⪯st.(mp_log)).
+  {
+    destruct Hcomp as [Hbad|Hcomp]; last done.
+    enough (log'=st.(mp_log)) by naive_solver.
+    symmetry.
+    by apply list_prefix_eq.
+  }
+  replace (st.(mp_acceptedEpoch)) with epoch' by word.
+
+  iDestruct (own_mono _ _
+               {[ epoch' := (◯ML _) ]}
+              with "Hacc_lb") as "$".
+  {
+    apply singleton_mono.
+    apply mono_list_lb_mono.
+    done.
+  }
+Qed.
 
 Lemma ghost_replica_accept_new_epoch γsys γsrv st epoch' log' :
   int.nat st.(mp_epoch) ≤ int.nat epoch' →
@@ -176,16 +446,111 @@ Lemma ghost_replica_accept_new_epoch γsys γsrv st epoch' log' :
   ==∗
   own_replica_ghost γsys γsrv (mkMPaxosState epoch' epoch' log').
 Proof.
-Admitted.
+  intros Hineq1 Hneq2.
+  iNamed 1.
+  iIntros "#Hprop_lb2 #Hprop_facts2".
+  assert (int.nat st.(mp_epoch) < int.nat epoch' ∨ int.nat st.(mp_epoch) = int.nat epoch') as Hcases.
+  { word. }
+  destruct Hcases as [HnewEpoch|HcurrentEpoch].
+  { (* case: mp_acceptedEpoch < mp_epoch == epoch'; get stuff out of Hunused *)
+    iClear "Hacc".
+    iDestruct (big_sepS_elem_of_acc_impl epoch' with "Hunused") as "[Hacc Hunused]".
+    { set_solver. }
+    iSpecialize ("Hacc" with "[%//]").
+    iMod (own_update with "Hacc") as "Hacc".
+    {
+      apply singleton_update.
+      apply mono_list_update.
+      instantiate (1:=log').
+      apply prefix_nil.
+    }
+    iModIntro.
+    iDestruct (own_mono _ _ {[ epoch' := (◯ML _) ]}
+                with "Hacc") as "#Hacc_lb2".
+    { apply singleton_mono. apply mono_list_included. }
+    unfold own_replica_ghost.
+    simpl.
+    destruct (decide _); last first.
+    { exfalso. done. }
+    iFrame "Hacc #".
+    iSplitR; first done.
+    iSplitR.
+    { iIntros (?). exfalso. lia. }
+    iSplitL "Hunused".
+    {
+      iApply "Hunused".
+      {
+        iModIntro.
+        iIntros (???) "Hwand".
+        iIntros (Hy).
+        iApply "Hwand".
+        iPureIntro. word.
+      }
+      {
+        iIntros.
+        exfalso. lia.
+      }
+    }
+    iApply (big_sepS_impl with "Hvotes").
+    iModIntro.
+    iIntros (??) "[%|$]".
+    iLeft.
+    iPureIntro. word.
+  }
+  { (* case: mp_acceptedEpoch < mp_epoch == epoch'; use existing acc *)
+    destruct (decide _).
+    { exfalso. word. }
 
-(* TODO: this is probably just the definition *)
+    iMod (own_update with "Hacc") as "Hacc".
+    {
+      apply singleton_update.
+      apply mono_list_update.
+      instantiate (1:=log').
+      apply prefix_nil.
+    }
+    iModIntro.
+    replace st.(mp_epoch) with (epoch') by word.
+    iDestruct (own_mono _ _ {[ epoch' := (◯ML _) ]}
+                with "Hacc") as "#Hacc_lb2".
+    { apply singleton_mono. apply mono_list_included. }
+
+    unfold own_replica_ghost.
+    simpl.
+    destruct (decide _); last first.
+    { exfalso. done. }
+    iFrame "Hacc #".
+    iSplitR; first done.
+    iSplitR.
+    { iIntros (?). exfalso. lia. }
+    iSplitL "Hunused".
+    {
+      iApply (big_sepS_impl with "Hunused").
+      iModIntro.
+      iIntros (??) "Hwand".
+      iIntros (?).
+      iApply "Hwand".
+      iPureIntro. word.
+    }
+    {
+      iApply (big_sepS_impl with "Hvotes").
+      iModIntro.
+      iIntros (??) "[%|$]".
+      iLeft.
+      iPureIntro. word.
+    }
+  }
+Qed.
+
+(* TODO: this is just the definition *)
 Lemma establish_committed_by epoch σ (W:gset nat) :
   (∀ s, s ∈ W → s < length config) →
   2 * (size W) > length config →
   ([∗ list] s0↦γsrv' ∈ config, ⌜s0 ∈ W⌝ → is_accepted_lb γsrv' epoch σ) -∗
   committed_by epoch σ.
 Proof.
-Admitted.
+  iIntros.
+  iExists _; iFrame "∗#%".
+Qed.
 
 Definition sys_inv γsys := inv sysN
 (
@@ -196,6 +561,7 @@ Definition sys_inv γsys := inv sysN
   is_proposal_facts γsys epoch σ
 ).
 
+(* copy/pasted almost verbatin from ghost_commit in pb_ghost.v! *)
 Lemma ghost_commit γsys epoch σ :
   sys_inv γsys -∗
   committed_by epoch σ -∗
@@ -204,17 +570,67 @@ Lemma ghost_commit γsys epoch σ :
   ={⊤}=∗ (* XXX: this is ⊤ because the user-provided fupd is fired, and it is allowed to know about ⊤ *)
   is_ghost_lb γsys σ.
 Proof.
-Admitted.
+  iIntros "#Hinv #Hcom #Hprop_lb #Hprop_facts".
+  iInv "Hinv" as "Hown" "Hclose".
+  iDestruct "Hown" as (σcommit epoch_commit) "(>Hghost & >#Hcom_com & >#Hprop_lb_com & #Hprop_facts_com)".
+  iDestruct "Hprop_facts_com" as "(>Hmax_com & Hvalid_com)".
+  iDestruct "Hprop_facts" as "(Hmax & Hvalid)".
+  iAssert (⌜σcommit ⪯ σ⌝ ∨ ⌜σ ⪯ σcommit⌝)%I as "%Hlog".
+  {
+    assert (int.nat epoch < int.nat epoch_commit ∨ int.nat epoch = int.nat epoch_commit ∨ int.nat epoch > int.nat epoch_commit) as [Hepoch|[Hepoch|Hepoch]]by word.
+    { (* case epoch < epoch_commit: use old_proposal_max of epoch_commit. *)
+      iRight.
+      by iApply "Hmax_com".
+    }
+    { (* case epoch = epoch_commit: proposal is comparable *)
+      replace (epoch) with (epoch_commit) by word.
+      iDestruct (own_valid_2 with "Hprop_lb Hprop_lb_com") as %Hvalid.
+      rewrite singleton_op in Hvalid.
+      rewrite singleton_valid in Hvalid.
+      apply mono_list_lb_op_valid_1_L in Hvalid.
+      iPureIntro.
+      naive_solver.
+    }
+    { (* case epoch_commit < epoch: use old_proposal_max of epoch *)
+      iLeft.
+      by iApply "Hmax".
+    }
+  }
 
-
-Definition is_accepted_upper_bound γsrv log (acceptedEpoch newEpoch:u64) : iProp Σ :=
-  ∃ logPrefix,
-  ⌜logPrefix ⪯ log⌝ ∗
-  is_accepted_ro γsrv acceptedEpoch logPrefix ∗
-  □ (∀ epoch', ⌜int.nat acceptedEpoch < int.nat epoch'⌝ -∗
-            ⌜int.nat epoch' < int.nat newEpoch⌝ -∗
-            is_accepted_ro γsrv epoch' [])
-.
+  destruct Hlog as [Hcan_update|Halready_updated].
+  {
+    iEval (unfold is_proposal_valid) in "Hvalid".
+    iDestruct ("Hvalid" $! σcommit with "[] Hghost") as "Hghost".
+    { done. }
+    iMod "Hghost".
+    unfold own_commit.
+    iEval (rewrite mono_list_auth_lb_op) in "Hghost".
+    iDestruct "Hghost" as "[Hghost $]".
+    iMod ("Hclose" with "[-]").
+    {
+      iNext.
+      iExists _, _. iFrame "∗".
+      iFrame "Hcom".
+      iFrame "#".
+    }
+    done.
+  }
+  {
+    unfold own_commit.
+    iEval (rewrite mono_list_auth_lb_op) in "Hghost".
+    iDestruct "Hghost" as "[Hghost #Hlb]".
+    iDestruct (own_mono with "Hlb") as "$".
+    {
+      by apply mono_list_lb_mono.
+    }
+    iMod ("Hclose" with "[-]").
+    {
+      iNext.
+      iExists _, _. iFrame "∗#".
+    }
+    done.
+  }
+Qed.
 
 Lemma is_accepted_upper_bound_mono_epoch γsrv log acceptedEpoch acceptedEpoch' newEpoch :
   int.nat acceptedEpoch < int.nat acceptedEpoch' →
@@ -252,7 +668,21 @@ Lemma is_accepted_upper_bound_mono_log γsrv log log' acceptedEpoch newEpoch :
   is_accepted_upper_bound γsrv log' acceptedEpoch newEpoch
 .
 Proof.
-Admitted.
+  intros Hle.
+  iIntros "Hacc_ub".
+  iDestruct "Hacc_ub" as (?) "(%Hpre & #Hro & #Hskip)".
+  iExists _; iFrame "Hro".
+  iSplitR.
+  {
+    iPureIntro.
+    by transitivity log.
+  }
+  iModIntro.
+  iIntros.
+  iApply "Hskip".
+  { iPureIntro. word. }
+  { iPureIntro. word. }
+Qed.
 
 Lemma is_proposal_lb_compare γsys log log' epoch :
   length log' ≤ length log →
@@ -261,17 +691,250 @@ Lemma is_proposal_lb_compare γsys log log' epoch :
   ⌜prefix log' log⌝
 .
 Proof.
+  intros Hlen.
+  iIntros "Hprop1 Hprop2".
+  iDestruct (own_valid_2 with "Hprop1 Hprop2") as %Hcomp.
+  rewrite singleton_op singleton_valid in Hcomp.
+  rewrite -Cinr_op Cinr_valid in Hcomp.
+  rewrite mono_list_lb_op_valid_L in Hcomp.
+  destruct Hcomp as [Hbad|Hcomp]; last done.
+  enough (log'=log) by naive_solver.
+  symmetry.
+  by apply list_prefix_eq.
+Qed.
+
+Definition validSet (W:gset nat) :=
+  ∀ s, s ∈ W → s < length config.
+
+Lemma validSet_union (W1 W2:gset nat) :
+  validSet W1 →
+  validSet W2 →
+  validSet (W1 ∪ W2).
+Proof.
+  intros.
+  intros ??.
+  apply elem_of_union in H1 as [|].
+  { naive_solver. }
+  { naive_solver. }
+Qed.
+
+(* TODO: THIS IS THE HARD LEMMA *)
+Lemma validSet_size (W:gset nat) :
+  validSet W →
+  size W ≤ length config.
+Proof.
 Admitted.
 
-Lemma become_leader γsys (W:gset nat) latestLog acceptedEpoch newEpoch:
+Definition vote_inv γsys := inv sysN
+(
+  [∗ set] e ∈ (fin_to_set u64),
+  (∃ (W:gset nat), ⌜validSet W⌝ ∗ ⌜2 * (size W) > length config⌝ ∗
+  [∗ list] s↦γsrv ∈ config, ⌜s ∈ W⌝ → own_vote_tok γsrv e) ∨
+  own_proposal γsys e []
+).
+
+Lemma quorum_overlap W1 W2 :
+  validSet W1 →
+  2 * (size W1) > length config →
+  validSet W2 →
+  2 * (size W2) > length config →
+  ∃ x γsrv, x ∈ W1 ∧ x ∈ W2 ∧
+            config !! x = Some γsrv
+.
+Proof.
+  intros HW Hquorum  HW2 Hquorum2.
+  destruct (decide ((W1 ∩ W2) = ∅)).
+  { (* case: the proposal has already been claimed; this should be impossible *)
+    exfalso.
+    pose proof (size_union W1 W2) as H.
+    assert (W1 ## W2).
+    { set_solver. }
+    apply H in H0.
+    pose proof (validSet_union _ _ HW HW2) as HuValid.
+    apply validSet_size in HuValid.
+    word.
+  }
+  {
+    apply set_choose_L in n.
+    destruct n as [s Hs].
+    apply elem_of_intersection in Hs as [HsW HsW2].
+    (* get a vote out of Hvotes1 and Hvotes2, then contradiction *)
+    assert (s < length config).
+    { apply HW. done. }
+    pose proof (list_lookup_lt _ _ _ H) as [γsrv' Hlookup].
+    exists s, γsrv'.
+    done.
+  }
+Qed.
+
+Lemma get_proposal_from_votes γsys (W:gset nat) newEpoch :
   2 * (size W) > length config →
+  validSet W →
+  vote_inv γsys -∗
+  ([∗ list] s↦γsrv ∈ config, ⌜s ∈ W⌝ → own_vote_tok γsrv newEpoch) ={↑sysN}=∗
+  own_proposal γsys newEpoch [].
+Proof.
+  intros Hquorum HW.
+  iIntros "#Hinv Hvotes".
+  iInv "Hinv" as ">Hi" "Hclose".
+  iDestruct (big_sepS_elem_of_acc_impl newEpoch with "Hi") as "[Hprop Hi]".
+  { set_solver. }
+  iDestruct "Hprop" as "[Hbad|Hprop]".
+  {
+    iDestruct "Hbad" as (W2) "(%HW2 & %Hquorum2 & Hvotes2)".
+    pose proof (quorum_overlap _ _ HW Hquorum HW2 Hquorum2) as [? [? [? []]]].
+
+    iDestruct (big_sepL_lookup_acc with "Hvotes") as "[Hvote1 _]".
+    { done. }
+    iSpecialize ("Hvote1" with "[%//]").
+    iDestruct (big_sepL_lookup_acc with "Hvotes2") as "[Hvote2 _]".
+    { done. }
+    iSpecialize ("Hvote2" with "[%//]").
+    iDestruct (own_valid_2 with "Hvote1 Hvote2") as %Hbad.
+    exfalso.
+    rewrite singleton_op in Hbad.
+    rewrite singleton_valid in Hbad.
+    apply dfrac_agree_op_valid_L in Hbad as [Hbad _].
+    done.
+  }
+  iFrame "Hprop".
+  iMod ("Hclose" with "[Hi Hvotes]").
+  {
+    iApply ("Hi" with "[] [Hvotes]").
+    {
+      iModIntro.
+      iIntros.
+      iFrame.
+    }
+    {
+      iLeft.
+      iExists _; iFrame.
+      done.
+    }
+  }
+  done.
+Qed.
+
+Lemma accepted_upper_bound_lb γsrv acceptedEpoch newEpoch log log':
+  is_accepted_lb γsrv acceptedEpoch log -∗
+  is_accepted_upper_bound γsrv log' acceptedEpoch newEpoch -∗
+  ⌜log ⪯ log'⌝
+.
+Proof.
+  iIntros "#Hacc_lb #Hacc_ub".
+  iDestruct "Hacc_ub" as (?) "(%Hpre & #Hacc_ro & Hacc_ub)".
+  iDestruct (own_valid_2 with "Hacc_ro Hacc_lb") as %Hvalid.
+  rewrite singleton_op singleton_valid in Hvalid.
+  rewrite mono_list_both_dfrac_valid_L in Hvalid.
+  destruct Hvalid as [_ [ Hvalid]].
+  iPureIntro.
+  assert (log ⪯ logPrefix).
+  {
+    rewrite H.
+    by apply prefix_app_r.
+  }
+  eapply transitivity.
+  { done. }
+  { done. }
+Qed.
+
+Lemma accepted_upper_bound_lb2 γsrv acceptedEpoch epoch newEpoch log log':
+  int.nat acceptedEpoch < int.nat epoch →
+  int.nat epoch < int.nat newEpoch →
+  is_accepted_lb γsrv epoch log -∗
+  is_accepted_upper_bound γsrv log' acceptedEpoch newEpoch -∗
+  ⌜log ⪯ log'⌝
+.
+Proof.
+  intros Hineq Hineq2.
+  iIntros "#Hacc_lb #Hacc_ub".
+  iDestruct "Hacc_ub" as (?) "(%Hpre & #Hacc_ro & #Hacc_ub)".
+  iSpecialize ("Hacc_ub" $! epoch with "[%//] [%//]").
+
+  iDestruct (own_valid_2 with "Hacc_ub Hacc_lb") as %Hvalid.
+  rewrite singleton_op singleton_valid in Hvalid.
+  rewrite mono_list_both_dfrac_valid_L in Hvalid.
+  destruct Hvalid as [_ [ Hvalid]].
+  iPureIntro.
+  symmetry in H.
+  apply app_eq_nil in H as [-> ].
+  apply prefix_nil.
+Qed.
+
+(* This is where the magic happens *)
+Lemma become_leader γsys (W:gset nat) latestLog acceptedEpoch newEpoch:
+  validSet W →
+  2 * (size W) > length config →
+  vote_inv γsys -∗
   ([∗ list] s↦γsrv ∈ config, ⌜s ∈ W⌝ → is_accepted_upper_bound γsrv latestLog acceptedEpoch newEpoch) -∗
+  is_proposal_lb γsys acceptedEpoch latestLog -∗
+  is_proposal_facts γsys acceptedEpoch latestLog -∗
   ([∗ list] s↦γsrv ∈ config, ⌜s ∈ W⌝ → own_vote_tok γsrv newEpoch) ={↑sysN}=∗
   own_leader_ghost γsys (mkMPaxosState newEpoch newEpoch latestLog)
 .
 Proof.
-Admitted.
+  intros HW Hquorum.
+  iIntros "#Hinv #Hacc #Hprop_lb #Hprop_facts Hvotes".
 
+  iMod (get_proposal_from_votes with "Hinv Hvotes") as "Hprop".
+  { done. }
+  { done. }
+
+  iMod (own_update with "Hprop") as "Hprop".
+  {
+    apply singleton_update.
+    apply csum_update_r.
+    apply mono_list_update.
+    instantiate (1:=latestLog).
+    apply prefix_nil.
+  }
+
+  iFrame "Hprop".
+  iDestruct "Hprop_facts" as "[Hmax Hvalid]".
+  iFrame "Hvalid".
+
+  (* establish old_proposal_max *)
+  iModIntro.
+  iIntros (?).
+  iModIntro.
+  simpl.
+  iIntros (? HepochIneq) "#Hcom_old".
+
+  destruct (decide (int.nat epoch_old < int.nat acceptedEpoch)).
+  { (* case: epoch_old < acceptedEpoch, just use prev old_prop_max *)
+    iApply "Hmax".
+    { done. }
+    iFrame "Hcom_old".
+  }
+
+  iDestruct "Hcom_old" as (W2) "(%HW2 & %Hquorum2 & Hcom_old)".
+  (* note that W and W2 overlap *)
+  pose proof (quorum_overlap _ _ HW Hquorum HW2 Hquorum2) as [? [? [? []]]].
+  iDestruct (big_sepL_lookup_acc with "Hacc") as "[Hacc_ub _ ]".
+  { done. }
+  iSpecialize ("Hacc_ub" with "[%//]").
+  iDestruct (big_sepL_lookup_acc with "Hcom_old") as "[Hacc_lb _]".
+  { done. }
+  iSpecialize ("Hacc_lb" with "[%//]").
+
+  destruct (decide (int.nat acceptedEpoch = int.nat epoch_old)).
+  { (* case: epoch_old = acceptedEpoch *)
+    replace (acceptedEpoch) with (epoch_old); last first.
+    {
+      assert (int.Z acceptedEpoch = int.Z epoch_old) by word.
+      naive_solver. (* XXX: why do I have to assert this Z inequalit? *)
+    } (* we have int.nat a = int.nat b, and need to show a = b *)
+    iDestruct (accepted_upper_bound_lb with "Hacc_lb Hacc_ub") as %Hineq.
+    done.
+  }
+  { (* case: acceptedEpoch < epoch_old < newEpoch *)
+    assert (int.nat acceptedEpoch < int.nat epoch_old) as Hineq by word.
+    iDestruct (accepted_upper_bound_lb2 with "Hacc_lb Hacc_ub") as %Hineq2.
+    { done. }
+    { done. }
+    done.
+  }
+Qed.
 
 Lemma ghost_leader_get_proposal γsys st :
   own_leader_ghost γsys st -∗
@@ -279,13 +942,25 @@ Lemma ghost_leader_get_proposal γsys st :
   is_proposal_facts γsys st.(mp_epoch) st.(mp_log)
 .
 Proof.
-Admitted.
+  iNamed 1.
+  iFrame "#".
+  iDestruct (own_mono with "Hprop") as "$".
+  {
+    apply singleton_included.
+    right.
+    apply Cinr_included.
+    apply mono_list_included.
+  }
+Qed.
 
 Lemma ghost_replica_helper1 γsys γsrv st :
   own_replica_ghost γsys γsrv st -∗
-  ⌜int.nat st.(mp_acceptedEpoch) < int.nat st.(mp_epoch)⌝.
+  ⌜int.nat st.(mp_acceptedEpoch) ≤ int.nat st.(mp_epoch)⌝.
 Proof.
-Admitted.
+  iNamed 1.
+  iPureIntro.
+  done.
+Qed.
 
 Lemma ghost_replica_enter_new_epoch γsys γsrv st newEpoch :
   int.nat newEpoch > int.nat st.(mp_epoch) →
@@ -297,6 +972,179 @@ Lemma ghost_replica_enter_new_epoch γsys γsrv st newEpoch :
   is_proposal_facts γsys st.(mp_acceptedEpoch) st.(mp_log)
 .
 Proof.
-Admitted.
+  intros Hineq.
+  iNamed 1.
+
+  (* FIXME: take points-tos out of Hunused, with e < newEpoch *)
+  set (F1:=(λ e, (⌜int.nat e > int.nat st.(mp_epoch)⌝ → ⌜int.nat e < int.nat newEpoch⌝ → own_accepted γsrv e []))%I).
+  set (F2:=(λ e, (⌜int.nat e > int.nat newEpoch⌝ → own_accepted γsrv e []))%I).
+  set (F3:=(λ e, (⌜int.nat e = int.nat newEpoch⌝ → own_accepted γsrv e []))%I).
+  iDestruct (big_sepS_impl with "Hunused []") as "Hunused".
+  {
+    instantiate (1:=(λ e, (F1 e ∗ F3 e) ∗ F2 e)%I).
+    iModIntro.
+    iIntros (??) "Hwand".
+    unfold F1. unfold F2. unfold F3.
+    destruct (decide (int.nat x < int.nat newEpoch)).
+    {
+      iSplitL "Hwand".
+      {
+        iSplitL "Hwand".
+        { iIntros. iApply "Hwand". iPureIntro. word. }
+        { iIntros. exfalso. word. }
+      }
+      { iIntros. exfalso. word. }
+    }
+    {
+      destruct (decide (int.nat x = int.nat newEpoch)).
+      {
+        iSplitL "Hwand".
+        {
+          iSplitR "Hwand".
+          { iIntros. exfalso. word. }
+          { iIntros. iApply "Hwand". iPureIntro. word. }
+        }
+        { iIntros. exfalso. word. }
+    }
+    {
+      assert (int.nat x > int.nat newEpoch) by word.
+      iSplitR "Hwand".
+      {
+        iSplitL.
+        { iIntros. exfalso. word. }
+        { iIntros. exfalso. word. }
+      }
+      { iIntros. iApply "Hwand". iPureIntro. word. }
+    }
+    }
+  }
+  simpl.
+  iDestruct (big_sepS_sep with "Hunused") as "[Hunused HunusedNew]".
+  unfold F2.
+  iDestruct (big_sepS_sep with "Hunused") as "[Hunused HunusedSingle]".
+  (* Now, we can do whatever we want with Hunused (F1); let's freeze it all! *)
+
+  set (G1:=(λ (e:u64),
+        |==> (⌜int.nat e > int.nat st.(mp_epoch)⌝
+          → ⌜int.nat e < int.nat newEpoch⌝ -∗
+          is_accepted_ro γsrv e [])%I
+                  )%I).
+  iDestruct (big_sepS_impl with "Hunused []") as "Hunused".
+  {
+    iModIntro.
+    instantiate (1:=G1).
+    iIntros (??) "Hwand".
+    unfold F1.
+    unfold G1.
+
+    destruct (decide (int.nat st.(mp_epoch) < int.nat x)); last first.
+    {
+      iModIntro.
+      iIntros. exfalso; word.
+    }
+    destruct (decide (int.nat x < int.nat newEpoch)); last first.
+    {
+      iModIntro.
+      iIntros. exfalso; word.
+    }
+    iSpecialize ("Hwand" with "[%//] [%//]").
+
+    iMod (own_update with "Hwand") as "$"; last done.
+    apply singleton_update.
+    apply mono_list_auth_persist.
+  }
+  unfold G1.
+  iMod (big_sepS_bupd with "Hunused") as "#Hunused".
+
+  iDestruct (big_sepS_elem_of_acc_impl newEpoch with "HunusedSingle") as "[Hacc2 _]".
+  { set_solver. }
+  iSpecialize ("Hacc2" with "[%//]").
+  iDestruct (big_sepS_elem_of_acc_impl newEpoch with "Hvotes") as "[Hvote Hvotes]".
+  { set_solver. }
+  iDestruct "Hvote" as "[%Hbad|Hvote]".
+  { exfalso. word. }
+
+  iAssert (|==> is_accepted_upper_bound γsrv st.(mp_log) st.(mp_acceptedEpoch) newEpoch)%I with "[Hacc Hunused]" as ">#Hacc_ub2".
+  {
+    destruct (decide _).
+    { (* case: need to freeze *)
+      iMod (own_update with "Hacc") as "Hacc".
+      {
+        apply singleton_update.
+        apply mono_list_auth_persist.
+      }
+      iDestruct "Hacc" as "#Hacc_ro".
+
+      iModIntro.
+      iExists st.(mp_log).
+      iSplit; first done.
+      replace st.(mp_epoch) with st.(mp_acceptedEpoch) by word.
+      iFrame "#".
+      iModIntro.
+      iIntros.
+      iDestruct (big_sepS_elem_of_acc_impl epoch' with "Hunused") as "[Hunused2 _]".
+      { set_solver. }
+      iApply "Hunused2".
+      { iPureIntro. word. }
+      { iPureIntro. word. }
+    }
+    {
+      iMod (own_update with "Hacc") as "Hacc".
+      {
+        apply singleton_update.
+        apply mono_list_auth_persist.
+      }
+      iDestruct "Hacc" as "#Hacc_ro".
+      iSpecialize ("Hacc_ub" with "[%]").
+      { word. }
+      iDestruct "Hacc_ub" as (?) "(%Hpre & #Hacc_ro2 & #Hacc_ub)".
+      iExists _.
+      iModIntro.
+      iSplit; first iPureIntro.
+      { done. }
+      iFrame "Hacc_ro2".
+      iModIntro.
+      iIntros.
+      destruct (decide (int.nat epoch' < int.nat st.(mp_epoch))).
+      { iApply "Hacc_ub"; done. }
+      assert (int.nat st.(mp_epoch) ≤ int.nat epoch') by word.
+
+      iDestruct (big_sepS_elem_of_acc_impl epoch' with "Hunused") as "[Hunused2 _]".
+      { set_solver. }
+      destruct (decide (int.nat epoch' = int.nat st.(mp_epoch))).
+      {
+        replace (epoch') with (st.(mp_epoch)) by word.
+        iFrame "#".
+      }
+      iApply "Hunused2".
+      { iPureIntro. word. }
+      { iPureIntro. word. }
+    }
+  }
+
+  iModIntro.
+  iFrame "Hvote".
+  iFrame "Hprop_lb Hprop_facts Hacc_lb".
+  simpl.
+  destruct (decide _).
+  { exfalso. word. }
+  iFrame "Hacc2".
+  iFrame "#".
+  iSplitR; first iPureIntro.
+  { word. }
+  iSplitR; first done.
+  iFrame "HunusedNew".
+  iApply "Hvotes".
+  {
+    iModIntro.
+    iIntros (???) "[%|$]".
+    iLeft.
+    iPureIntro. word.
+  }
+  {
+    iLeft.
+    iPureIntro. word.
+  }
+Qed.
 
 End mpaxos_protocol.
